theories/Minimax_Rule_Ref.thy
@@ -26,7 +26,7 @@ subsection \<open>Correctness\<close>
 lemma minimax_rule_imp_correct:
   shows "(uncurry minimax_rule_imp, uncurry (RETURN 
     oo (minimax_rule:: (nat Electoral_Module))))
-  \<in> elec_mod_seprel nat_assn"
+  \<in> elec_mod_seprel id_assn"
   using minimax_rule_imp.refine
   unfolding minimax_rule.simps elector_opt_eq
   .
@@ -35,7 +35,7 @@ declare minimax_rule_imp_correct [sepref_fr_rules]
 
 subsection \<open>Properties in Separation Logic\<close>
 
-theorem pmc_impl_condorcet:
+theorem minimax_rule_imp_condorcet:
   shows "finite_profile A p \<and> condorcet_winner A p w \<Longrightarrow>
   <(alts_set_impl_assn nat_assn) A hs *
             (list_assn (ballot_assn nat_assn)) p hp> minimax_rule_imp hs hp 
